git-svn-id: https://projects.brucker.ch/hol-testgen/svn/HOL-TestGen/trunk/hol-testgen@10541 3260e6d1-4efc-4170-b0a7-36055960796d

src/OCL_collection_type_Pair.thy
@@ -47,51 +47,7 @@ theory  OCL_collection_type_Pair
 imports OCL_basic_type
 begin
 
-section{* Complex Types: The Pair-Collection Type (I) Core *}
-
-subsection{* The Construction of the Pair Type (Tuples) *}
-
-text{* The core of an own type construction is done via a type
-  definition which provides the base-type @{text "('\<alpha>, '\<beta>) Pair\<^sub>b\<^sub>a\<^sub>s\<^sub>e"}. It
-  is shown that this type ``fits'' indeed into the abstract type
-  interface discussed in the previous section. *}
-
-typedef ('\<alpha>, '\<beta>) Pair\<^sub>b\<^sub>a\<^sub>s\<^sub>e = "{X::('\<alpha>\<Colon>null \<times> '\<beta>\<Colon>null) option option.
-                                       X = bot \<or> X = null \<or> (fst\<lceil>\<lceil>X\<rceil>\<rceil> \<noteq> bot \<and> snd\<lceil>\<lceil>X\<rceil>\<rceil> \<noteq> bot)}"
-                          by (rule_tac x="bot" in exI, simp)
-
-
-instantiation   Pair\<^sub>b\<^sub>a\<^sub>s\<^sub>e  :: (null,null)bot
-begin
-   definition bot_Pair\<^sub>b\<^sub>a\<^sub>s\<^sub>e_def: "(bot_class.bot :: ('a\<Colon>null,'b\<Colon>null) Pair\<^sub>b\<^sub>a\<^sub>s\<^sub>e) \<equiv> Abs_Pair\<^sub>b\<^sub>a\<^sub>s\<^sub>e None"
-
-   instance proof show "\<exists>x\<Colon>('a,'b) Pair\<^sub>b\<^sub>a\<^sub>s\<^sub>e. x \<noteq> bot"
-                  apply(rule_tac x="Abs_Pair\<^sub>b\<^sub>a\<^sub>s\<^sub>e \<lfloor>None\<rfloor>" in exI)
-                  apply(simp add:bot_Pair\<^sub>b\<^sub>a\<^sub>s\<^sub>e_def)
-                  apply(subst Abs_Pair\<^sub>b\<^sub>a\<^sub>s\<^sub>e_inject)
-                  apply(simp_all add: bot_Pair\<^sub>b\<^sub>a\<^sub>s\<^sub>e_def
-                                      null_option_def bot_option_def)
-                  done
-            qed
-end
-
-instantiation   Pair\<^sub>b\<^sub>a\<^sub>s\<^sub>e  :: (null,null)null
-begin
-   definition null_Pair\<^sub>b\<^sub>a\<^sub>s\<^sub>e_def: "(null::('a::null,'b::null) Pair\<^sub>b\<^sub>a\<^sub>s\<^sub>e) \<equiv> Abs_Pair\<^sub>b\<^sub>a\<^sub>s\<^sub>e \<lfloor> None \<rfloor>"
-
-   instance proof show "(null::('a::null,'b::null) Pair\<^sub>b\<^sub>a\<^sub>s\<^sub>e) \<noteq> bot"
-                  apply(simp add:null_Pair\<^sub>b\<^sub>a\<^sub>s\<^sub>e_def bot_Pair\<^sub>b\<^sub>a\<^sub>s\<^sub>e_def)
-                  apply(subst Abs_Pair\<^sub>b\<^sub>a\<^sub>s\<^sub>e_inject)
-                  apply(simp_all add: bot_Pair\<^sub>b\<^sub>a\<^sub>s\<^sub>e_def null_option_def bot_option_def)
-                  done
-            qed
-end
-
-
-text{* ...  and lifting this type to the format of a valuation gives us:*}
-type_synonym    ('\<AA>,'\<alpha>,'\<beta>) Pair  = "('\<AA>, ('\<alpha>,'\<beta>) Pair\<^sub>b\<^sub>a\<^sub>s\<^sub>e) val"
-
-section{* Complex Types: The Pair-Collection Type (II) Library *}
+section{* Complex Types: The Collection Pair-Type Operations *}
 
 text{* This part provides a collection of operators for the Pair type. *}
 
